semantics/fpSemScript.sml
@@ -53,7 +53,7 @@ val _ = Hol_datatype `
 
 (*val fp_cmp : fp_cmp -> word64 -> word64 -> bool*)
 val _ = Define `
- ((fp_cmp:fp_cmp -> word64 -> word64 -> bool) fop=  ((case fop of
+ (fp_cmp fop=  ((case fop of
     FP_Less => fp64_lessThan
   | FP_LessEqual => fp64_lessEqual
   | FP_Greater => fp64_greaterThan
@@ -64,7 +64,7 @@ val _ = Define `
 
 (*val fp_uop : fp_uop -> word64 -> word64*)
 val _ = Define `
- ((fp_uop:fp_uop -> word64 -> word64) fop=  ((case fop of
+ (fp_uop fop=  ((case fop of
     FP_Abs => fp64_abs
   | FP_Neg => fp64_negate
   | FP_Sqrt => fp64_sqrt roundTiesToEven
@@ -73,7 +73,7 @@ val _ = Define `
 
 (*val fp_bop : fp_bop -> word64 -> word64 -> word64*)
 val _ = Define `
- ((fp_bop:fp_bop -> word64 -> word64 -> word64) fop=  ((case fop of
+ (fp_bop fop=  ((case fop of
     FP_Add => fp64_add roundTiesToEven
   | FP_Sub => fp64_sub roundTiesToEven
   | FP_Mul => fp64_mul roundTiesToEven
@@ -82,12 +82,12 @@ val _ = Define `
 
 
 val _ = Define `
- ((fpfma:word64 -> word64 -> word64 -> word64) v1 v2 v3=  (fp64_mul_add roundTiesToEven v2 v3 v1))`;
+ (fpfma v1 v2 v3=  (fp64_mul_add roundTiesToEven v2 v3 v1))`;
 
 
 (*val fp_top : fp_top -> word64 -> word64 -> word64 -> word64*)
 val _ = Define `
- ((fp_top:fp_top -> word64 -> word64 -> word64 -> word64) fop=  ((case fop of
+ (fp_top fop=  ((case fop of
     FP_Fma => fpfma
 )))`;
 
